Part 1

Using y – y1 = m(x – x1) to find the intersection point.

 $\y – y_1 = m_1*(x – x_1)$ -> point nr 1
\- $\y – y_2 = m_2*(x – x_2)$ -> point nr 2
------------------------
  $\y_2 - y_1 = m_1*x - m_1* x_1 - m_2*x + m_2 * x_2$

                         ||
                        \  /
                         \/

$\x = (y_1 - y_2 - m_1 * x_1 + m_2 * x_2) / (m_2 - m_1)$
$\y = m_1*(x – x_1) + y_1$

Part 2
Assuming that if a thrown rock at time "t" hits another rock then:
$\x_r + t * v_xr = x_1 + t * v_x1$
so $\t = (x_r - x_1) / (v_x1 - v_xr)$
and comparing x with y there is equazotion:
$\(x_r - x_1) / (v_x1 - v_xr) = (y_r - y_1) / (v_y1 - v_yr)$
so $\(v_y2-v_y1) * x_r + (v_x1-v_x2) * y_r + (y_1-y_2) * v_xr + (x_1-x_2) * v_yr = x_2* v_y2 - y_2 * v_x2 - x_2 * v_y1 + y_1 * v_x1$
